Added MIN constant to top_level_ctx

language/tests/coq/ConcordiumImpls.v
@@ -9,12 +9,8 @@ Require Import Hacspec.Lib.
 
 Notation "'reject'" := (int32) : hacspec_scope.
 
-Definition iint32_min  : int32 :=
-  (not (@repr WORDSIZE32 0)) .^ (@cast _ int32 _ ((not (
-          @repr WORDSIZE32 0)) shift_right (usize 1))).
-
 Definition reject_impl_default  : reject :=
-  iint32_min .
+  min.
 
 Inductive option_reject :=
 | SomeReject : reject -> option_reject
@@ -25,20 +21,35 @@ Definition new_reject_impl (x_0 : int32) : option_reject :=
       NoneReject)).
 
 Definition reject_impl_convert_from_unit  : reject :=
-  (iint32_min ) .+ (@repr WORDSIZE32 1).
+  (min) .+ (@repr WORDSIZE32 1).
+
+Theorem ensures_reject_impl_convert_from_unit : forall result_1 ,
+ @reject_impl_convert_from_unit  = result_1 ->
+ (result_1) !=.? (@repr WORDSIZE32 0).
+ Proof. Admitted.
 
 Definition reject_impl_convert_from_parse_error  : reject :=
-  (iint32_min ) .+ (@repr WORDSIZE32 2).
+  (min) .+ (@repr WORDSIZE32 2).
+
+Theorem ensures_reject_impl_convert_from_parse_error : forall result_1 ,
+ @reject_impl_convert_from_parse_error  = result_1 ->
+ (result_1) !=.? (@repr WORDSIZE32 0).
+ Proof. Admitted.
 
 Inductive log_error :=
 | Full : log_error
 | Malformed : log_error.
 
-Definition reject_impl_from_log_error (le_1 : log_error) : reject :=
-  match le_1 with
-  | Full => (iint32_min ) .+ (@repr WORDSIZE32 3)
-  | Malformed => (iint32_min ) .+ (@repr WORDSIZE32 4)
+Definition reject_impl_from_log_error (le_2 : log_error) : reject :=
+  match le_2 with
+  | Full => (min) .+ (@repr WORDSIZE32 3)
+  | Malformed => (min) .+ (@repr WORDSIZE32 4)
   end.
+
+Theorem ensures_reject_impl_from_log_error : forall result_1 (le_2 : log_error),
+ @reject_impl_from_log_error le_2 = result_1 ->
+ (result_1) !=.? (@repr WORDSIZE32 0).
+ Proof. Admitted.
 
 Inductive new_contract_name_error :=
 | NewContractNameErrorMissingInitPrefix : new_contract_name_error
@@ -47,16 +58,20 @@ Inductive new_contract_name_error :=
 | NewContractNameErrorInvalidCharacters : new_contract_name_error.
 
 Definition reject_impl_from_new_contract_name_error
-  (nre_2 : new_contract_name_error)
+  (nre_3 : new_contract_name_error)
   : reject :=
-  match nre_2 with
-  | NewContractNameErrorMissingInitPrefix => (iint32_min ) .+ (
-    @repr WORDSIZE32 5)
-  | NewContractNameErrorTooLong => (iint32_min ) .+ (@repr WORDSIZE32 6)
-  | NewContractNameErrorContainsDot => (iint32_min ) .+ (@repr WORDSIZE32 9)
-  | NewContractNameErrorInvalidCharacters => (iint32_min ) .+ (
-    @repr WORDSIZE32 10)
+  match nre_3 with
+  | NewContractNameErrorMissingInitPrefix => (min) .+ (@repr WORDSIZE32 5)
+  | NewContractNameErrorTooLong => (min) .+ (@repr WORDSIZE32 6)
+  | NewContractNameErrorContainsDot => (min) .+ (@repr WORDSIZE32 9)
+  | NewContractNameErrorInvalidCharacters => (min) .+ (@repr WORDSIZE32 10)
   end.
+
+Theorem ensures_reject_impl_from_new_contract_name_error : forall result_1 (
+  nre_3 : new_contract_name_error),
+ @reject_impl_from_new_contract_name_error nre_3 = result_1 ->
+ (result_1) !=.? (@repr WORDSIZE32 0).
+ Proof. Admitted.
 
 Inductive new_receive_name_error :=
 | NewReceiveNameErrorMissingDotSeparator : new_receive_name_error
@@ -64,15 +79,19 @@ Inductive new_receive_name_error :=
 | NewReceiveNameErrorInvalidCharacters : new_receive_name_error.
 
 Definition reject_impl_from_new_receive_name_error
-  (nre_3 : new_receive_name_error)
+  (nre_4 : new_receive_name_error)
   : reject :=
-  match nre_3 with
-  | NewReceiveNameErrorMissingDotSeparator => (iint32_min ) .+ (
-    @repr WORDSIZE32 7)
-  | NewReceiveNameErrorTooLong => (iint32_min ) .+ (@repr WORDSIZE32 8)
-  | NewReceiveNameErrorInvalidCharacters => (iint32_min ) .+ (
-    @repr WORDSIZE32 11)
+  match nre_4 with
+  | NewReceiveNameErrorMissingDotSeparator => (min) .+ (@repr WORDSIZE32 7)
+  | NewReceiveNameErrorTooLong => (min) .+ (@repr WORDSIZE32 8)
+  | NewReceiveNameErrorInvalidCharacters => (min) .+ (@repr WORDSIZE32 11)
   end.
+
+Theorem ensures_reject_impl_from_new_receive_name_error : forall result_1 (
+  nre_4 : new_receive_name_error),
+ @reject_impl_from_new_receive_name_error nre_4 = result_1 ->
+ (result_1) !=.? (@repr WORDSIZE32 0).
+ Proof. Admitted.
 
 Notation "'contract_state'" := (int32) : hacspec_scope.
 
@@ -90,153 +109,153 @@ Notation "'uint32_option'" := ((option int32)) : hacspec_scope.
 Notation "'iint64_option'" := ((option int64)) : hacspec_scope.
 
 Definition contract_state_impl_seek
-  (current_position_4 : contract_state)
-  (pos_5 : seek_from)
+  (current_position_5 : contract_state)
+  (pos_6 : seek_from)
   : (contract_state × seek_result) :=
-  match pos_5 with
-  | Start offset_6 => (@cast _ uint32 _ (offset_6), SeekResultOk (offset_6))
-  | End delta_7 => (if ((delta_7) >=.? (@repr WORDSIZE64 0)):bool then (
-      match pub_uint32_checked_add (current_position_4) (@cast _ uint32 _ (
-          delta_7)) with
-      | Some b_8 => (b_8, SeekResultOk (@cast _ uint64 _ (delta_7)))
-      | None => (current_position_4, SeekResultErr (tt))
-      end) else (match pub_int64_checked_abs (delta_7) with
-      | Some b_9 => (
-        (@repr WORDSIZE32 4) .- (@cast _ uint32 _ (b_9)),
+  match pos_6 with
+  | Start offset_7 => (@cast _ uint32 _ (offset_7), SeekResultOk (offset_7))
+  | End delta_8 => (if ((delta_8) >=.? (@repr WORDSIZE64 0)):bool then (
+      match pub_uint32_checked_add (current_position_5) (@cast _ uint32 _ (
+          delta_8)) with
+      | Some b_9 => (b_9, SeekResultOk (@cast _ uint64 _ (delta_8)))
+      | None => (current_position_5, SeekResultErr (tt))
+      end) else (match pub_int64_checked_abs (delta_8) with
+      | Some b_10 => (
+        (@repr WORDSIZE32 4) .- (@cast _ uint32 _ (b_10)),
         SeekResultOk (@cast _ uint64 _ ((@repr WORDSIZE32 4) .- (
-              @cast _ uint32 _ (b_9))))
+              @cast _ uint32 _ (b_10))))
       )
-      | None => (current_position_4, SeekResultErr (tt))
+      | None => (current_position_5, SeekResultErr (tt))
       end))
-  | Current delta_10 => (if ((delta_10) >=.? (@repr WORDSIZE64 0)):bool then (
-      match pub_uint32_checked_add (current_position_4) (@cast _ uint32 _ (
-          delta_10)) with
-      | Some offset_11 => (
-        offset_11,
-        SeekResultOk (@cast _ uint64 _ (offset_11))
+  | Current delta_11 => (if ((delta_11) >=.? (@repr WORDSIZE64 0)):bool then (
+      match pub_uint32_checked_add (current_position_5) (@cast _ uint32 _ (
+          delta_11)) with
+      | Some offset_12 => (
+        offset_12,
+        SeekResultOk (@cast _ uint64 _ (offset_12))
       )
-      | None => (current_position_4, SeekResultErr (tt))
-      end) else (match pub_int64_checked_abs (delta_10) with
-      | Some b_12 => match pub_uint32_checked_sub (current_position_4) (
-        @cast _ uint32 _ (b_12)) with
-      | Some offset_13 => (
-        offset_13,
-        SeekResultOk (@cast _ uint64 _ (offset_13))
+      | None => (current_position_5, SeekResultErr (tt))
+      end) else (match pub_int64_checked_abs (delta_11) with
+      | Some b_13 => match pub_uint32_checked_sub (current_position_5) (
+        @cast _ uint32 _ (b_13)) with
+      | Some offset_14 => (
+        offset_14,
+        SeekResultOk (@cast _ uint64 _ (offset_14))
       )
-      | None => (current_position_4, SeekResultErr (tt))
+      | None => (current_position_5, SeekResultErr (tt))
       end
-      | None => (current_position_4, SeekResultErr (tt))
+      | None => (current_position_5, SeekResultErr (tt))
       end))
   end.
 
 Definition contract_state_impl_read_read
-  (current_position_14 : contract_state)
-  (num_read_15 : int32)
+  (current_position_15 : contract_state)
+  (num_read_16 : int32)
   : (contract_state × uint_size) :=
-  ((current_position_14) .+ (num_read_15), @cast _ uint32 _ (num_read_15)).
+  ((current_position_15) .+ (num_read_16), @cast _ uint32 _ (num_read_16)).
 
 Definition contract_state_impl_read_read_u64
-  (current_position_16 : contract_state)
-  (num_read_17 : int32)
+  (current_position_17 : contract_state)
+  (num_read_18 : int32)
   : (contract_state × bool) :=
   (
-    (current_position_16) .+ (num_read_17),
-    (num_read_17) =.? (@repr WORDSIZE32 8)
+    (current_position_17) .+ (num_read_18),
+    (num_read_18) =.? (@repr WORDSIZE32 8)
   ).
 
 Definition contract_state_impl_read_read_u32
-  (current_position_18 : contract_state)
-  (num_read_19 : int32)
+  (current_position_19 : contract_state)
+  (num_read_20 : int32)
   : (contract_state × bool) :=
   (
-    (current_position_18) .+ (num_read_19),
-    (num_read_19) =.? (@repr WORDSIZE32 4)
+    (current_position_19) .+ (num_read_20),
+    (num_read_20) =.? (@repr WORDSIZE32 4)
   ).
 
 Definition contract_state_impl_read_read_u8
-  (current_position_20 : contract_state)
-  (num_read_21 : int32)
+  (current_position_21 : contract_state)
+  (num_read_22 : int32)
   : (contract_state × bool) :=
   (
-    (current_position_20) .+ (num_read_21),
-    (num_read_21) =.? (@repr WORDSIZE32 1)
+    (current_position_21) .+ (num_read_22),
+    (num_read_22) =.? (@repr WORDSIZE32 1)
   ).
 
 Definition write_impl_for_contract_state_test
-  (current_position_22 : contract_state)
-  (len_23 : int32)
+  (current_position_23 : contract_state)
+  (len_24 : int32)
   : bool :=
-  option_is_none (pub_uint32_checked_add (current_position_22) (len_23)).
+  option_is_none (pub_uint32_checked_add (current_position_23) (len_24)).
 
 Definition write_impl_for_contract_state
-  (current_position_24 : contract_state)
-  (num_bytes_25 : int32)
+  (current_position_25 : contract_state)
+  (num_bytes_26 : int32)
   : (contract_state × uint_size) :=
-  ((current_position_24) .+ (num_bytes_25), @cast _ uint32 _ (num_bytes_25)).
+  ((current_position_25) .+ (num_bytes_26), @cast _ uint32 _ (num_bytes_26)).
 
 Definition has_contract_state_impl_for_contract_state_open  : contract_state :=
   @repr WORDSIZE32 0.
 
 Definition has_contract_state_impl_for_contract_state_reserve_0
-  (len_26 : int32)
-  (cur_size_27 : int32)
+  (len_27 : int32)
+  (cur_size_28 : int32)
   : bool :=
-  (cur_size_27) <.? (len_26).
+  (cur_size_28) <.? (len_27).
 
 Definition has_contract_state_impl_for_contract_state_reserve_1
-  (res_28 : int32)
+  (res_29 : int32)
   : bool :=
-  (res_28) =.? (@repr WORDSIZE32 1).
+  (res_29) =.? (@repr WORDSIZE32 1).
 
 Definition has_contract_state_impl_for_contract_state_truncate_0
-  (cur_size_29 : int32)
-  (new_size_30 : int32)
+  (cur_size_30 : int32)
+  (new_size_31 : int32)
   : bool :=
-  (cur_size_29) >.? (new_size_30).
+  (cur_size_30) >.? (new_size_31).
 
 Definition has_contract_state_impl_for_contract_state_truncate_1
-  (current_position_31 : contract_state)
-  (new_size_32 : int32)
+  (current_position_32 : contract_state)
+  (new_size_33 : int32)
   : contract_state :=
-  (if ((new_size_32) <.? (current_position_31)):bool then (new_size_32) else (
-      current_position_31)).
+  (if ((new_size_33) <.? (current_position_32)):bool then (new_size_33) else (
+      current_position_32)).
 
 Notation "'parameter'" := (int32) : hacspec_scope.
 
 Definition read_impl_for_parameter_read
-  (current_position_33 : parameter)
-  (num_read_34 : int32)
+  (current_position_34 : parameter)
+  (num_read_35 : int32)
   : (parameter × uint_size) :=
-  ((current_position_33) .+ (num_read_34), @cast _ uint32 _ (num_read_34)).
+  ((current_position_34) .+ (num_read_35), @cast _ uint32 _ (num_read_35)).
 
 Notation "'attributes_cursor'" := ((int32 × int16)) : hacspec_scope.
 
 Definition has_policy_impl_for_policy_attributes_cursor_next_test
-  (policy_attribute_items_35 : attributes_cursor)
+  (policy_attribute_items_36 : attributes_cursor)
   : bool :=
-  let '(_, remaining_items_36) :=
-    policy_attribute_items_35 in 
-  (remaining_items_36) =.? (@repr WORDSIZE16 0).
+  let '(_, remaining_items_37) :=
+    policy_attribute_items_36 in 
+  (remaining_items_37) =.? (@repr WORDSIZE16 0).
 
 Definition has_policy_impl_for_policy_attributes_cursor_next_tag_invalid
-  (policy_attribute_items_37 : attributes_cursor)
-  (tag_value_len_1_38 : int8)
-  (num_read_39 : int32)
+  (policy_attribute_items_38 : attributes_cursor)
+  (tag_value_len_1_39 : int8)
+  (num_read_40 : int32)
   : (attributes_cursor × bool) :=
-  let '(current_position_40, remaining_items_41) :=
-    policy_attribute_items_37 in 
-  let policy_attribute_items_42 : (int32 × int16) :=
-    ((current_position_40) .+ (num_read_39), remaining_items_41) in 
-  (policy_attribute_items_42, (tag_value_len_1_38) >.? (@repr WORDSIZE8 31)).
+  let '(current_position_41, remaining_items_42) :=
+    policy_attribute_items_38 in 
+  let policy_attribute_items_43 : (int32 × int16) :=
+    ((current_position_41) .+ (num_read_40), remaining_items_42) in 
+  (policy_attribute_items_43, (tag_value_len_1_39) >.? (@repr WORDSIZE8 31)).
 
 Definition has_policy_impl_for_policy_attributes_cursor_next
-  (policy_attribute_items_43 : attributes_cursor)
-  (num_read_44 : int32)
+  (policy_attribute_items_44 : attributes_cursor)
+  (num_read_45 : int32)
   : attributes_cursor :=
-  let '(current_position_45, remaining_items_46) :=
-    policy_attribute_items_43 in 
+  let '(current_position_46, remaining_items_47) :=
+    policy_attribute_items_44 in 
   (
-    (current_position_45) .+ (num_read_44),
-    (remaining_items_46) .- (@repr WORDSIZE16 1)
+    (current_position_46) .+ (num_read_45),
+    (remaining_items_47) .- (@repr WORDSIZE16 1)
   ).
 
